Changed BreadthFirstSearch example to no longer use "inductive naturals", sequences, or roll-it-yourself maps.  Instead, use "nat", List, and "map". Use VC splitting to combat performance issues.

Test/vstte2012/BreadthFirstSearch.dfy
@@ -6,15 +6,14 @@ class BreadthFirstSearch<Vertex(==)>
 
   // This is the definition of what it means to be a path "p" from vertex 
   // "source" to vertex "dest"
-  function IsPath(source: Vertex, dest: Vertex, p: seq<Vertex>): bool
+  predicate IsPath(source: Vertex, dest: Vertex, p: List<Vertex>)
   {
-    if source == dest then
-      p == []
-    else
-      p != [] && dest in Succ(p[|p|-1]) && IsPath(source, p[|p|-1], p[..|p|-1])
+    match p
+    case Nil => source == dest
+    case Cons(v, tail) => dest in Succ(v) && IsPath(source, v, tail)
   }
 
-  function IsClosed(S: set<Vertex>): bool  // says that S is closed under Succ
+  predicate IsClosed(S: set<Vertex>)  // says that S is closed under Succ
   {
     forall v :: v in S ==> Succ(v) <= S
   }
@@ -25,7 +24,7 @@ class BreadthFirstSearch<Vertex(==)>
   // witness.  The method could equally well have been written using an 
   // existential quantifier and no ghost out-parameter.
   method BFS(source: Vertex, dest: Vertex, ghost AllVertices: set<Vertex>) 
-         returns (d: int, ghost path: seq<Vertex>)
+         returns (d: int, ghost path: List<Vertex>)
     // source and dest are among AllVertices
     requires source in AllVertices && dest in AllVertices;  
     // AllVertices is closed under Succ
@@ -34,14 +33,15 @@ class BreadthFirstSearch<Vertex(==)>
     // More precisely, "d" is non-negative iff "source" can reach "dest".
     // The following postcondition says that under the "0 <= d" outcome, 
     // "path" denotes a path of length "d" from "source" to "dest":
-    ensures 0 <= d ==> IsPath(source, dest, path) && |path| == d;
+    ensures 0 <= d ==> IsPath(source, dest, path) && length(path) == d;
     // Moreover, that path is as short as any path from "source" to "dest":
-    ensures 0 <= d ==> forall p :: IsPath(source, dest, p) ==> |path| <= |p|;
+    ensures 0 <= d ==> forall p :: IsPath(source, dest, p) ==> length(path) <= length(p);
     // Finally, under the outcome "d < 0", there is no path from "source" to "dest":
     ensures d < 0 ==> !exists p :: IsPath(source, dest, p);
   {
     var V, C, N := {source}, {source}, {};
-    ghost var Processed, paths := {}, Maplet({source}, source, [], Empty);
+    ghost var Processed, paths := {}, map[source := Nil];
+    assert domain(paths) == {source};
     // V - all encountered vertices
     // Processed - vertices reachable from "source" is at most "d" steps
     // C - unprocessed vertices reachable from "source" in "d" steps 
@@ -49,8 +49,7 @@ class BreadthFirstSearch<Vertex(==)>
     // N - vertices encountered and reachable from "source" in "d+1" steps 
     //     (but no less)
     d := 0;
-    var dd := Zero;
-    while (C != {})
+    while C != {}
       // V, Processed, C, N are all subsets of AllVertices:
       invariant V <= AllVertices && Processed <= AllVertices && C <= AllVertices && N <= AllVertices;
       // source is encountered:
@@ -60,20 +59,18 @@ class BreadthFirstSearch<Vertex(==)>
       invariant Processed !! C !! N;  // Processed, C, and N are mutually disjoint
       // "paths" records a path for every encountered vertex
       invariant ValidMap(source, paths);
-      invariant V == Domain(paths);
+      invariant V == domain(paths);
       // shortest paths for vertices in C have length d, and for vertices in N
       // have length d+1
-      invariant forall x :: x in C ==> |Find(source, x, paths)| == d;
-      invariant forall x :: x in N ==> |Find(source, x, paths)| == d + 1;
-      // "dd" is just an inductive-looking way of writing "d":
-      invariant Value(dd) == d;
+      invariant forall x :: x in C ==> length(Find(source, x, paths)) == d;
+      invariant forall x :: x in N ==> length(Find(source, x, paths)) == d + 1;
       // "dest" is not reachable for any smaller value of "d":
-      invariant dest in R(source, dd, AllVertices) ==> dest in C;
-      invariant d != 0 ==> dest !in R(source, dd.predecessor, AllVertices);
+      invariant dest in R(source, d, AllVertices) ==> dest in C;
+      invariant d != 0 ==> dest !in R(source, d-1, AllVertices);
       // together, Processed and C are all the vertices reachable in at most d steps:
-      invariant Processed + C == R(source, dd, AllVertices);
+      invariant Processed + C == R(source, d, AllVertices);
       // N are the successors of Processed that are not reachable within d steps:
-      invariant N == Successors(Processed, AllVertices) - R(source, dd, AllVertices);
+      invariant N == Successors(Processed, AllVertices) - R(source, d, AllVertices);
       // if we have exhausted C, then we have also exhausted N:
       invariant C == {} ==> N == {};
       // variant:
@@ -84,15 +81,14 @@ class BreadthFirstSearch<Vertex(==)>
       C, Processed := C - {v}, Processed + {v};
       ghost var pathToV := Find(source, v, paths);
     
-      if (v == dest) {
+      if v == dest {
         forall p | IsPath(source, dest, p)
-          ensures |pathToV| <= |p|;
+          ensures length(pathToV) <= length(p);
         {
           Lemma_IsPath_R(source, dest, p, AllVertices);
-          if (|p| < |pathToV|) {
+          if length(p) < length(pathToV) {
             // show that this branch is impossible
-            ToNat_Value_Bijection(|p|);
-            RMonotonicity(source, ToNat(|p|), dd.predecessor, AllVertices);
+            RMonotonicity(source, length(p), d-1, AllVertices);
           }
         }
         return d, pathToV;
@@ -103,20 +99,20 @@ class BreadthFirstSearch<Vertex(==)>
       V, N := V + newlyEncountered, N + newlyEncountered;
       paths := UpdatePaths(newlyEncountered, source, paths, v, pathToV);
 
-      if (C == {}) {
-        C, N, d, dd := N, {}, d+1, Suc(dd);
+      if C == {} {
+        C, N, d := N, {}, d+1;
       }
     }
 
     // show that "dest" in not in any reachability set, no matter 
     // how many successors one follows
-    forall nn
-      ensures dest !in R(source, nn, AllVertices);
+    forall n: nat
+      ensures dest !in R(source, n, AllVertices);
     {
-      if (Value(nn) < Value(dd)) {
-        RMonotonicity(source, nn, dd, AllVertices);
+      if n < d {
+        RMonotonicity(source, n, d, AllVertices);
       } else {
-        IsReachFixpoint(source, dd, nn, AllVertices);
+        IsReachFixpoint(source, d, n, AllVertices);
       }
     }
 
@@ -129,7 +125,7 @@ class BreadthFirstSearch<Vertex(==)>
     {
       Lemma_IsPath_R(source, dest, p, AllVertices);
       // a consequence of Lemma_IsPath_R is:  
-      // dest in R(source, ToNat(|p|), AllVertices)
+      // dest in R(source, |p|), AllVertices)
       // but that contradicts the conclusion of the preceding forall statement
     }
 
@@ -138,46 +134,24 @@ class BreadthFirstSearch<Vertex(==)>
 
   // property of IsPath
 
-  ghost method Lemma_IsPath_Closure(source: Vertex, dest: Vertex, 
-                                p: seq<Vertex>, AllVertices: set<Vertex>)
+  lemma Lemma_IsPath_Closure(source: Vertex, dest: Vertex, 
+                             p: List<Vertex>, AllVertices: set<Vertex>)
     requires IsPath(source, dest, p) && source in AllVertices && IsClosed(AllVertices);
-    ensures dest in AllVertices && forall v :: v in p ==> v in AllVertices;
+    ensures dest in AllVertices && forall v :: v in elements(p) ==> v in AllVertices;
   {
-    if (p != []) {
-      var last := |p| - 1;
-      Lemma_IsPath_Closure(source, p[last], p[..last], AllVertices);
+    match p {
+      case Nil =>
+      case Cons(v, tail) =>
+        Lemma_IsPath_Closure(source, v, tail, AllVertices);
     }
-  }
-
-  // operations on Nat
-
-  function Value(nn: Nat): nat
-    ensures ToNat(Value(nn)) == nn;
-  {
-    match nn
-    case Zero => 0
-    case Suc(mm) => Value(mm) + 1
-  }
-
-  function ToNat(n: nat): Nat
-  {
-    if n == 0 then Zero else Suc(ToNat(n - 1))
-  }
-
-  ghost method ToNat_Value_Bijection(n: nat)
-    ensures Value(ToNat(n)) == n;
-  {
-    // Dafny automatically figures out the inductive proof of the postcondition
   }
 
   // Reachability
 
-  function R(source: Vertex, nn: Nat, AllVertices: set<Vertex>): set<Vertex>
+  function R(source: Vertex, n: nat, AllVertices: set<Vertex>): set<Vertex>
   {
-    match nn
-    case Zero => {source}
-    case Suc(mm) =>  R(source, mm, AllVertices) + 
-                     Successors(R(source, mm, AllVertices), AllVertices)
+    if n == 0 then {source} else
+    R(source, n-1, AllVertices) + Successors(R(source, n-1, AllVertices), AllVertices)
   }
 
   function Successors(S: set<Vertex>, AllVertices: set<Vertex>): set<Vertex>
@@ -185,92 +159,94 @@ class BreadthFirstSearch<Vertex(==)>
     set w | w in AllVertices && exists x :: x in S && w in Succ(x)
   }
 
-  ghost method RMonotonicity(source: Vertex, mm: Nat, nn: Nat, AllVertices: set<Vertex>)
-    requires Value(mm) <= Value(nn);
-    ensures R(source, mm, AllVertices) <= R(source, nn, AllVertices);
-    decreases Value(nn) - Value(mm);
+  lemma RMonotonicity(source: Vertex, m: nat, n: nat, AllVertices: set<Vertex>)
+    requires m <= n;
+    ensures R(source, m, AllVertices) <= R(source, n, AllVertices);
+    decreases n - m;
   {
-    if (Value(mm) < Value(nn)) {
-      RMonotonicity(source, Suc(mm), nn, AllVertices);
+    if m < n {
+      RMonotonicity(source, m + 1, n, AllVertices);
     }
   }
 
-  ghost method IsReachFixpoint(source: Vertex, mm: Nat, nn: Nat, AllVertices: set<Vertex>)
-    requires R(source, mm, AllVertices) == R(source, Suc(mm), AllVertices);
-    requires Value(mm) <= Value(nn);
-    ensures R(source, mm, AllVertices) == R(source, nn, AllVertices);
-    decreases Value(nn) - Value(mm);
+  lemma IsReachFixpoint(source: Vertex, m: nat, n: nat, AllVertices: set<Vertex>)
+    requires R(source, m, AllVertices) == R(source, m+1, AllVertices);
+    requires m <= n;
+    ensures R(source, m, AllVertices) == R(source, n, AllVertices);
+    decreases n - m;
   {
-    if (Value(mm) < Value(nn)) {
-      IsReachFixpoint(source, Suc(mm), nn, AllVertices);
+    if m < n {
+      IsReachFixpoint(source, m + 1, n, AllVertices);
     }
   }
 
-  ghost method Lemma_IsPath_R(source: Vertex, x: Vertex, 
-                              p: seq<Vertex>, AllVertices: set<Vertex>)
+  lemma Lemma_IsPath_R(source: Vertex, x: Vertex, p: List<Vertex>, AllVertices: set<Vertex>)
     requires IsPath(source, x, p) && source in AllVertices && IsClosed(AllVertices);
-    ensures x in R(source, ToNat(|p|), AllVertices);
+    ensures x in R(source, length(p), AllVertices);
   {
-    if (p != []) {
-      Lemma_IsPath_Closure(source, x, p, AllVertices);
-      var last := |p| - 1;
-      Lemma_IsPath_R(source, p[last], p[..last], AllVertices);
+    match p {
+      case Nil =>
+      case Cons(v, tail) =>
+        Lemma_IsPath_Closure(source, x, p, AllVertices);
+        Lemma_IsPath_R(source, v, tail, AllVertices);
     }
-  }
-
-  // operations on Map's
-
-  function Domain(m: Map<Vertex>): set<Vertex>
-  {
-//    if m.Maplet? then m.dom else {}
-//    if m == Empty then {} else assert m.Maplet?; m.dom
-    match m
-    case Empty => {}
-    case Maplet(dom, t, s, nxt) => dom
   }
 
   // ValidMap encodes the consistency of maps (think, invariant).
   // An explanation of this idiom is explained in the README file.
-  function ValidMap(source: Vertex, m: Map<Vertex>): bool
+  predicate ValidMap(source: Vertex, m: map<Vertex, List<Vertex>>)
   {
-    match m
-    case Empty =>  true
-    case Maplet(dom, v, path, next) =>
-      v in dom && dom == Domain(next) + {v} &&
-      IsPath(source, v, path) &&
-      ValidMap(source, next)
+    forall v :: v in m ==> IsPath(source, v, m[v])
   }
 
-  function Find(source: Vertex, x: Vertex, m: Map<Vertex>): seq<Vertex>
-    requires ValidMap(source, m) && x in Domain(m);
+  function Find(source: Vertex, x: Vertex, m: map<Vertex, List<Vertex>>): List<Vertex>
+    requires ValidMap(source, m) && x in m;
     ensures IsPath(source, x, Find(source, x, m));
   {
-    match m
-    case Maplet(dom, v, path, next) =>
-      if x == v then path else Find(source, x, next)
+    m[x]
   }
 
   ghost method UpdatePaths(vSuccs: set<Vertex>, source: Vertex, 
-                    paths: Map<Vertex>, v: Vertex, pathToV: seq<Vertex>) 
-               returns (newPaths: Map<Vertex>)
+                           paths: map<Vertex, List<Vertex>>, v: Vertex, pathToV: List<Vertex>) 
+               returns (newPaths: map<Vertex, List<Vertex>>)
     requires ValidMap(source, paths);
-    requires vSuccs !! Domain(paths);
-    requires forall succ :: succ in vSuccs ==> IsPath(source, succ, pathToV + [v]);
-    ensures ValidMap(source, newPaths) && Domain(newPaths) == Domain(paths) + vSuccs;
-    ensures forall x :: x in Domain(paths) ==> 
+    requires vSuccs !! domain(paths);
+    requires forall succ :: succ in vSuccs ==> IsPath(source, succ, Cons(v, pathToV));
+    ensures ValidMap(source, newPaths) && domain(newPaths) == domain(paths) + vSuccs;
+    ensures forall x :: x in paths ==> 
                         Find(source, x, paths) == Find(source, x, newPaths);
-    ensures forall x :: x in vSuccs ==> Find(source, x, newPaths) == pathToV + [v];
+    ensures forall x :: x in vSuccs ==> Find(source, x, newPaths) == Cons(v, pathToV);
   {
-    if (vSuccs == {}) {
+    if vSuccs == {} {
       newPaths := paths;
     } else {
       var succ :| succ in vSuccs;
-      newPaths := Maplet(Domain(paths) + {succ}, succ, pathToV + [v], paths);
+      newPaths := paths[succ := Cons(v, pathToV)];
+      assert domain(newPaths) == domain(paths) + {succ};
       newPaths := UpdatePaths(vSuccs - {succ}, source, newPaths, v, pathToV);
     }
   }
 }
 
-datatype Map<T> = Empty | Maplet(dom: set<T>, T, seq<T>, next: Map<T>);
+static function domain<T, U>(m: map<T, U>): set<T>
+{
+  set t | t in m
+}
 
-datatype Nat = Zero | Suc(predecessor: Nat);
+datatype List<T> = Nil | Cons(head: T, tail: List)
+
+static function length(list: List): nat
+{
+  match list
+  case Nil => 0
+  case Cons(_, tail) => 1 + length(tail)
+}
+
+static function elements<T>(list: List<T>): set<T>
+{
+  match list
+  case Nil => {}
+  case Cons(x, tail) => {x} + elements(tail)
+}
+
+datatype Nat = Zero | Suc(predecessor: Nat)
