Test/vstte2012/runtest.bat
@@ -4,7 +4,11 @@ setlocal
 set BINARIES=..\..\Binaries
 set DAFNY_EXE=%BINARIES%\Dafny.exe
 
-%DAFNY_EXE% /compile:0 /dprint:out.dfy.tmp /verifySeparately %* Two-Way-Sort.dfy Combinators.dfy RingBuffer.dfy RingBufferAuto.dfy Tree.dfy BreadthFirstSearch.dfy
+%DAFNY_EXE% /compile:0 /dprint:out.dfy.tmp /verifySeparately %* Two-Way-Sort.dfy Combinators.dfy RingBuffer.dfy RingBufferAuto.dfy Tree.dfy
+
+echo.
+echo -------------------- BreadthFirstSearch.dfy --------------------
+%DAFNY_EXE% /compile:0 /dprint:out.dfy.tmp /vcsMaxKeepGoingSplits:10 %* BreadthFirstSearch.dfy
 
 rem for %%f in (
 rem     Two-Way-Sort.dfy
